Add JSON parser (wip)

Monads.lean
@@ -1,4 +1,28 @@
 
+abbrev ℕ := Nat
+
+def randRange₀ (n : Nat) : Nat :=
+  sorry
+
+theorem reflexivity : ∀ (r : ℕ), r = r := by
+  intro r
+  rfl
+
+theorem rand_theorem (n : Nat) : randRange₀ n = randRange₀ n :=
+  reflexivity (randRange₀ n)
+
+-- So .... we are only going to be able to have constant random numbers with
+-- this signature !!!
+
+def randRange (n : Nat) : IO Nat :=
+  IO.Process.run {
+    cmd := "python",
+    args := #[
+      "-c",
+      s!"import random; print(random.randrange(0, {n}), end='')"
+    ]
+  } >>= (· |> String.toNat! |> pure)
+
 
 #eval "0x" ++ String.mk (Nat.toDigits 16 255)
 
@@ -29,6 +53,41 @@ def hex := hex₁
 #eval hex 4096
 -- "0x1000"
 
+def a := {
+  cmd := "python3", args := #["-c"]
+  : IO.Process.SpawnArgs
+}
+
+def strip_python (s : String) : IO String :=
+  let python_code := s!"print('{s}'.strip(), end='')"
+  let spawnArgs : IO.Process.SpawnArgs := {
+    cmd := "python", args := #["-c", python_code]
+  }
+  IO.Process.run spawnArgs
+
+#eval strip_python "  Hello world!  "
+-- "Hello world!"
+
+#eval strip_python "0x42\n"
+-- process 'python' exited with code 1 !
+
+def hex_python₀ (n : Nat) : IO String :=
+  let python_code := s!"print(hex({n}))"
+  let spawnArgs : IO.Process.SpawnArgs := {
+    cmd := "python", args := #["-c", python_code]
+  }
+  IO.Process.run spawnArgs >>= strip_python
+
+#eval hex_python₀
+-- "0x2a"
+
+def hex_python₉  (n : Nat) : IO String := do
+  let python_code := s!"print(hex({n}))"
+  let spawnArgs := { cmd := "python3", args := #["-c", python_code] }
+  let out ← IO.Process.run spawnArgs
+  return out.trim
+
+#eval hex_python 42
 
 def one_plus_one_python : IO String := do
   let spawnArgs := { cmd := "python3", args := #["-c", "print(1+1)"] }
