Json.lean
@@ -1,0 +1,300 @@
+
+
+
+namespace v0
+/-
+
+  - Objective: parse "null" as a JSON data structure.
+
+  - Use an inductive type to represent
+    the JSON data structure
+
+  - deriving repr for convenience.
+
+  - Come up with the idea of using an option type to represent results
+    or failure to parse when needed.
+
+-/
+
+inductive Json
+| null : Json
+deriving Repr
+
+def parseNull (input : String): Option Json :=
+  if input == "null" then
+    some Json.null
+  else
+    none
+
+def Json.parse := parseNull
+
+#eval Json.parse "null"
+-- some (v0.Json.null)
+
+#eval Json.parse "true"
+-- none
+
+#eval Json.parse "null null"
+-- none
+
+#eval Json.parse "  null"
+-- none
+
+end v0
+
+namespace v1
+
+inductive Json
+| null : Json
+| bool (b : Bool) : Json
+deriving Repr
+
+def parseNull (input : String): Option Json :=
+  if input == "null" then
+    some Json.null
+  else
+    none
+
+def parseBool (input : String): Option Json :=
+  if input == "true" then
+    some (Json.bool true)
+  else if input == "false" then
+    some (Json.bool false)
+  else
+    none
+
+def Json.parse (input : String): Option Json :=
+  match parseNull input with
+  | some json => some json
+  | none => parseBool input
+
+-- We see the beginning of a nesting pattern here that we'd like a solution
+-- to but it's not the usual "return none as soon as you get one" that is
+-- nicely encapsulated in the do notation. This is a "try this and if it
+-- fails, try that" pattern.
+
+#eval Json.parse "null"
+-- some (v1.Json.null)
+
+
+#eval Json.parse "false"
+-- some (v1.Json.bool false)
+
+#eval Json.parse "true"
+-- some (v1.Json.bool true)
+
+#eval Json.parse "null null"
+-- none
+
+#eval Json.parse "  null"
+-- none
+
+end v1
+
+
+namespace v2
+
+inductive Json
+| null : Json
+| bool (b : Bool) : Json
+deriving Repr
+
+def parseNull (input : String): Option Json :=
+  if input == "null" then
+    some Json.null
+  else
+    none
+
+def parseBool (input : String): Option Json :=
+  if input == "true" then
+    some (Json.bool true)
+  else if input == "false" then
+    some (Json.bool false)
+  else
+    none
+
+def Json.parse (input : String) : Option Json := -- orElse pattern
+   parseNull input <|> parseBool input
+
+#eval Json.parse "null"
+-- some (v2.Json.null)
+
+
+#eval Json.parse "false"
+-- some (v2.Json.bool false)
+
+#eval Json.parse "true"
+-- some (v2.Json.bool true)
+
+#eval Json.parse "null null"
+-- none
+
+#eval Json.parse "  null"
+-- none
+
+end v2
+
+
+namespace v3
+
+/-
+Preparing the introduction of arrays and/or whitespace;
+facing the issue that we need to change the signature
+of our parser to account for some *partial* success in the
+parsing of the input string.
+
+Not a big deal since we can generically build a "total parser" on top of
+a partial one if needed.
+
+-/
+
+inductive Json
+| null : Json
+| bool (b : Bool) : Json
+deriving Repr
+
+def parseNull (input : String): Option (Json × String) :=
+  if input.startsWith "null" then
+    some (Json.null, input.drop 4)
+  else
+    none
+
+def parseBool (input : String): Option (Json × String) :=
+  if input == "true" then
+    some (Json.bool true, input.drop 4)
+  else if input == "false" then
+    some (Json.bool false, input.drop 5)
+  else
+    none
+
+def Json.parse (input : String) : Option (Json × String) :=
+   parseNull input <|> parseBool input
+
+def parseEverything (parser : String → Option (Json × String)) (input : String) : Option Json :=
+  match parser input with
+  | some (json, rest) => if rest == "" then some json else none
+  | none => none
+
+#eval Json.parse "null"
+-- some (v3.Json.null, "")
+
+#eval parseEverything Json.parse "null"
+-- some (v3.Json.null)
+
+#eval Json.parse "null and more"
+-- some (v3.Json.null, " and more")
+
+#eval parseEverything Json.parse "null and more"
+-- none
+
+#eval Json.parse "false"
+-- some (v3.Json.bool false, "")
+
+#eval Json.parse "true"
+-- some (v3.Json.bool true, "")
+
+#eval Json.parse "null null"
+-- some (v3.Json.null, " null")
+
+#eval Json.parse "  null"
+-- none
+
+end v3
+
+namespace v4
+/-
+Introduction of arrays (without whitespace). -> Need for mutually recursive
+functions!
+-/
+
+inductive Json
+| null : Json
+| bool (b : Bool) : Json
+| array (elements : List Json) : Json
+deriving Repr
+
+def parseNull (input : String): Option (Json × String) :=
+  if input.startsWith "null" then
+    some (Json.null, input.drop 4)
+  else
+    none
+
+def parseBool (input : String): Option (Json × String) :=
+  if input == "true" then
+    some (Json.bool true, input.drop 4)
+  else if input == "false" then
+    some (Json.bool false, input.drop 5)
+  else
+    none
+
+-- -- We need a more generic version of parseEverything
+-- def parseEverything (parser : String → Option (α × String)) (input : String) : Option α :=
+--   match parser input with
+--   | some (json, rest) => if rest == "" then some json else none
+--   | none => none
+
+mutual
+
+  partial def parseValues (input : String) : Option (List Json × String) :=
+  sorry -- we need that to be greedy too, right?
+
+  partial def parseArray (input : String) : Option (Json × String) :=
+    if input.startsWith "[" then
+      match parseValues (input.drop 1) with
+      | none => none
+      | some (elements, rest) =>
+        if rest.startsWith "]" then
+          return (Json.array elements, rest.drop 1)
+        else
+          none
+    else
+      none
+
+  partial def Json.parse (input : String) : Option (Json × String) :=
+    parseNull input <|> parseBool input <|> parseArray input
+
+end
+
+def parseEverything (parser : String → Option (Json × String)) (input : String) : Option Json :=
+  match parser input with
+  | some (json, rest) => if rest == "" then some json else none
+  | none => none
+
+#eval Json.parse "null"
+-- some (v4.Json.null, "")
+
+#eval parseEverything Json.parse "null"
+-- some (v4.Json.null)
+
+#eval Json.parse "null and more"
+-- some (v4.Json.null, " and more")
+
+#eval parseEverything Json.parse "null and more"
+-- none
+
+#eval Json.parse "false"
+-- some (v4.Json.bool false, "")
+
+#eval Json.parse "true"
+-- some (v4.Json.bool true, "")
+
+#eval Json.parse "null null"
+-- some (v4.Json.null, " null")
+
+#eval Json.parse "  null"
+-- none
+
+end v4
+
+namespace v5
+/-
+Parse whitespace. Two important concept here:
+  - in the JSON spec, whitespace is actually *optional* whitespace :
+    "" is some whitespace
+  - we need our whitespace to match as much as possible (greedyness)
+
+Arf, fuck our whitespace is not represented in the Json structure,
+it needs a different signature. Actually can we just use trimLeft?
+Does it match the JSON spec?
+-/
+end v5
